src/common/Curve25519_Spec.ec
@@ -1,9 +1,11 @@
 require import List Int Int IntDiv CoreMap Real.
-from Jasmin require import JModel.
 require import Zp_25519.
-import Zp_25519.
 
-op decodeScalar25519 (k:W256.t) =
+from Jasmin require import JModel.
+
+import Zp_25519.Zp.
+
+op spec_decode_scalar_25519 (k:W256.t) =
     let k = k.[0   <- false] in
     let k = k.[1   <- false] in
     let k = k.[2   <- false] in
@@ -11,9 +13,9 @@ op decodeScalar25519 (k:W256.t) =
     let k = k.[254 <- true ] in
         k.
 
-op decodeUCoordinate (u:W256.t) = inzp (to_uint u).
+op spec_decode_u_coordinate (u:W256.t) = inzp (to_uint u).
 
-op add_and_double (qx : zp) (nqs : (zp * zp) * (zp * zp)) =
+op spec_add_and_double (qx : zp) (nqs : (zp * zp) * (zp * zp)) =
     let x_1 = qx                                      in
     let (x_2, z_2) = nqs.`1                           in
     let (x_3, z_3) = nqs.`2                           in
@@ -32,31 +34,31 @@ op add_and_double (qx : zp) (nqs : (zp * zp) * (zp * zp)) =
     let z_2        = e    *  (aa + (inzp 121665 * e)) in
         ((x_2, z_2), (x_3, z_3)).
 
-op swap_tuple (t : ('a * 'a) * ('a * 'a)) = (t.`2, t.`1).
+op spec_swap_tuple (t : ('a * 'a) * ('a * 'a)) = (t.`2, t.`1).
 
-op ith_bit    (k : W256.t, i : int)       = k.[i].
+op spec_ith_bit    (k : W256.t, i : int)       = k.[i].
 
-op montgomery_ladder (init: zp, k: W256.t)         =
-    let nqs0 = ((Zp_25519.one, Zp_25519.zero), (init, Zp_25519.one)) in
-        foldl (fun (nqs : (zp * zp) * (zp * zp)) ctr => 
-             if ith_bit k ctr
-                 then swap_tuple (add_and_double init (swap_tuple(nqs)))
-             else add_and_double init nqs) nqs0 (rev (iota_ 0 255)).
+op spec_montgomery_ladder (init: zp, k: W256.t)         =
+    let nqs0 = ((Zp.one, Zp.zero), (init, Zp.one)) in
+        foldl (fun (nqs : (zp * zp) * (zp * zp)) ctr =>
+             if spec_ith_bit k ctr
+                 then spec_swap_tuple (spec_add_and_double init (spec_swap_tuple(nqs)))
+             else spec_add_and_double init nqs) nqs0 (rev (iota_ 0 255)).
 
-op encodePoint (q: zp * zp) : W256.t  =
+op spec_encode_point (q: zp * zp) : W256.t  =
     let q = q.`1 * (ZModpRing.exp q.`2 (p - 2)) in
-        W256.of_int (asint q)                   axiomatized by encodePointE.
+        W256.of_int (asint q)                   axiomatized by spec_encode_pointE.
 
-op scalarmult_internal (k: zp) (u: W256.t) : W256.t =
-   let r = montgomery_ladder k u                in
-       encodePoint (r.`1)                       axiomatized by scalarmult_internalE. 
+op spec_scalarmult_internal (k: zp) (u: W256.t) : W256.t =
+   let r = spec_montgomery_ladder k u                in
+       spec_encode_point (r.`1)                       axiomatized by scalarmult_internalE.
 
-op scalarmult (k: W256.t) (u: W256.t) : W256.t =
-    let k = decodeScalar25519 k                 in
-    let u = decodeUCoordinate u                 in
-        scalarmult_internal u k                 axiomatized by scalarmultE. 
+op spec_scalarmult (k: W256.t) (u: W256.t) : W256.t =
+    let k = spec_decode_scalar_25519 k                 in
+    let u = spec_decode_u_coordinate u                 in
+        spec_scalarmult_internal u k                 axiomatized by spec_scalarmultE.
 
-hint simplify scalarmultE.
+hint simplify spec_scalarmultE.
 
-op scalarmult_base (k:W256.t) : W256.t =
-    scalarmult (k) (W256.of_int(9%Int)).
+op spec_scalarmult_base (k:W256.t) : W256.t =
+    spec_scalarmult (k) (W256.of_int(9%Int)).
