src/mulx/Curve25519_auto_mulx.ec
@@ -1,29 +1,25 @@
-require import Int Bool Zp_25519 List.
-require import Curve25519_Spec.
-require import Curve25519_Hop1.
-require import Curve25519_Hop2.
-require import Curve25519_mulx.
-require import W64limbs.
+require import Int StdOrder Ring IntDiv Bool List Real BitEncoding.
+require import Zp_25519 W64limbs Zplimbs Curve25519_Spec Curve25519_Procedures Curve25519_mulx.
 
-from Jasmin require import JWord JWord_array.
+from Jasmin require import JWord JWord_array JModel JUtils.
 
-import Zp_25519 Curve25519_Spec Curve25519_Hop2 Curve25519_mulx Array4 Array32.
+import Zp_25519.Zp Curve25519_Procedures Curve25519_mulx Array4 Array32 Ring.IntID StdOrder.IntOrder Array4.
 
 (* Probably needs to be moved elsewhere, such as W64limbs *)
 
 (** step 0 : add sub mul sqr - all done by auto **)
 
-equiv eq_h4_add_rrs_mulx : MHop2.add ~ M_mulx.__add4_rrs:
+equiv eq_spec_impl_add_rrs_mulx : CurveProcedures.add ~ M_mulx.__add4_rrs:
     f{1}   = inzpRep4 f{2} /\
     g{1}   = inzpRep4 g{2}
     ==>
     res{1} = inzpRep4 res{2}.
-proof. 
-    proc *.  
+proof.
+    proc *.
     admit.
 qed.
 
-equiv eq_h4_sub_rrs_mulx : MHop2.sub ~ M_mulx.__sub4_rrs:
+equiv eq_spec_impl_sub_rrs_mulx : CurveProcedures.sub ~ M_mulx.__sub4_rrs:
    f{1}   = inzpRep4 f{2} /\
    g{1}   = inzpRep4 gs{2}
    ==>
@@ -34,19 +30,19 @@ proof.
 qed.
 
 
-equiv eq_h4_sub_rsr_mulx : MHop2.sub ~ M_mulx.__sub4_rsr:
+equiv eq_spec_impl_sub_rsr_mulx : CurveProcedures.sub ~ M_mulx.__sub4_rsr:
    f{1}   = inzpRep4 fs{2} /\
    g{1}   = inzpRep4 g{2}
    ==>
    res{1} = inzpRep4 res{2}.
 proof.
-    proc *. 
+    proc *.
     admit.
 qed.
 
 (* inline mul4_c0 mul4_c1 mul4_c2 mul4_c3 *)
 
-equiv eq_h4_mul_a24_mulx : MHop2.mul_a24 ~ M_mulx.__mul4_a24_rs:
+equiv eq_spec_impl_mul_a24_mulx : CurveProcedures.mul_a24 ~ M_mulx.__mul4_a24_rs:
     f{1}   = inzpRep4 fs{2} /\
     a24{1} = to_uint a24{2}
     ==>
@@ -56,7 +52,7 @@ proof.
     admit.
 qed.
 
-equiv eq_h4_mul_rsr_mulx : MHop2.mul ~ M_mulx.__mul4_rsr:
+equiv eq_spec_impl_mul_rsr_mulx : CurveProcedures.mul ~ M_mulx.__mul4_rsr:
     f{1}   = inzpRep4 fs{2} /\
     g{1}   = inzpRep4 g{2}
     ==>
@@ -66,49 +62,49 @@ proof.
     admit.
 qed.
 
-equiv eq_h4_mul__rpr_mulx : MHop2.mul ~ M_mulx.__mul4_rpr:
+equiv eq_spec_impl_mul__rpr_mulx : CurveProcedures.mul ~ M_mulx.__mul4_rpr:
     f{1}   = inzpRep4 fp{2} /\
     g{1}   = inzpRep4 g{2}
     ==>
     res{1} = inzpRep4 res{2}.
 proof.
-    proc *.  
+    proc *.
     admit.
 qed.
 
-equiv eq_h4__sqr_rr_mulx : MHop2.sqr ~ M_mulx.__sqr4_rr:
+equiv eq_spec_impl__sqr_rr_mulx : CurveProcedures.sqr ~ M_mulx.__sqr4_rr:
     f{1}   = inzpRep4 f{2}
     ==>
     res{1} = inzpRep4 res{2}.
 proof.
-    proc *.  
+    proc *.
     admit.
 qed.
 
 (** step 1 : decode_scalar_25519 **)
-equiv eq_h4_decode_scalar_25519_mulx : MHop2.decode_scalar ~ M_mulx.__decode_scalar:
+equiv eq_spec_impl_decode_scalar_25519_mulx : CurveProcedures.decode_scalar ~ M_mulx.__decode_scalar:
     inzp (W256.to_uint k'{1})  = inzpRep4 k{2}
-    ==> 
-    inzp (W256.to_uint res{1}) = inzpRep32 res{2}. 
+    ==>
+    inzp (W256.to_uint res{1}) = inzpRep32 res{2}.
 proof.
     admit. (* AUTO *)
 qed.
 
 
 (** step 2 : decode_u_coordinate **)
-equiv eq_h4_decode_u_coordinate_mulx : MHop2.decode_u_coordinate ~ M_mulx.__decode_u_coordinate4:
+equiv eq_spec_impl_decode_u_coordinate_mulx : CurveProcedures.decode_u_coordinate ~ M_mulx.__decode_u_coordinate4:
     inzp (W256.to_uint u'{1}) = inzpRep4 u{2}
-    ==> 
+    ==>
     res{1}                    = inzpRep4 res{2}.
 proof.
     admit. (* AUTO MSB already 0 -  ask tiago *)
 qed.
 
 (** step 3 : ith_bit **)
-equiv eq_h4_ith_bit_mulx : MHop2.ith_bit ~ M_mulx.__ith_bit :
-    inzp (W256.to_uint k'{1}) = inzpRep32 k{2} /\  
-    (ctr{1}                   = to_uint ctr{2}) 
-    ==> 
+equiv eq_spec_impl_ith_bit_mulx : CurveProcedures.ith_bit ~ M_mulx.__ith_bit :
+    inzp (W256.to_uint k'{1}) = inzpRep32 k{2} /\
+    (ctr{1}                   = to_uint ctr{2})
+    ==>
     b2i res{1}                = to_uint res{2}.
 proof.
     proc.
@@ -117,13 +113,11 @@ qed.
 
 
 (** step 10 : encode point **)
-equiv eq_h4_encode_point_mulx : MHop2.encode_point ~ M_mulx.__encode_point4:
-    x2{1}                 = inzpRep4 x2{2} /\ 
+equiv eq_spec_impl_encode_point_mulx : CurveProcedures.encode_point ~ M_mulx.__encode_point4:
+    x2{1}                 = inzpRep4 x2{2} /\
     z2{1}                 = inzpRep4 z2r{2}
     ==>
     inzp (to_uint res{1}) = inzpRep4 res{2}.
 proof.
     admit. (* AUTO *)
 qed.
-    
-
