src/ref4/CorrectnessProof.ec
@@ -1,96 +1,92 @@
-require import AllCore Bool List Int IntDiv StdOrder CoreMap Real Zp_25519 Ring EClib Distr.
+require import AllCore Bool List Int IntDiv StdOrder CoreMap Real Zp_25519 Ring Distr.
+
 from Jasmin require import JModel JMemory JWord.
-require import Curve25519_Spec.
-require import Curve25519_Hop1.
-require import Curve25519_Hop2.
-require import Curve25519_Hop3.
-require import Curve25519_Ref4.
-require import Curve25519_auto4.
-require import W64limbs.
-import Zp_25519.
-import Curve25519_Spec Curve25519_auto4 Curve25519_Hop1 Curve25519_Hop2 Curve25519_Ref4 Array4 Array8 Array32 StdOrder.IntOrder.
+
+require import Curve25519_Procedures Curve25519_auto4 Curve25519_Ref4 W64limbs Zp_25519 Zplimbs EClib.
+
+import Zp_25519.Zp Curve25519_auto4 Curve25519_Procedures Curve25519_Ref4 Array4 Array8 Array32 StdOrder.IntOrder EClib.
 
 
 
 (* additions, substractions and powers *)
 
 (* additions, substractions and powers *)
-equiv eq_h4_add_ssr_ref4 : MHop2.add ~ M_ref4.__add4_ssr:
+equiv eq_spec_impl_add_ssr_ref4 : CurveProcedures.add ~ M_ref4.__add4_ssr:
     f{1}   = inzpRep4 g{2} /\
     g{1}   = inzpRep4 fs{2}
     ==>
     res{1} = inzpRep4 res{2}.
 proof.
     proc *. inline{2} (1). wp. sp.
-    call (eq_h4_add_rrs_ref4). skip. auto => />.
+    call (eq_spec_impl_add_rrs_ref4). skip. auto => />.
 qed.
 
 
-equiv eq_h4_add_sss_ref4 : MHop2.add ~ M_ref4.__add4_sss:
+equiv eq_spec_impl_add_sss_ref4 : CurveProcedures.add ~ M_ref4.__add4_sss:
     f{1}   = inzpRep4 fs{2} /\
     g{1}   = inzpRep4 gs{2}
     ==>
     res{1} = inzpRep4 res{2}.
 proof.
     proc *. inline{2} (1). wp. sp.
-    call eq_h4_add_rrs_ref4. skip. auto => />.
+    call eq_spec_impl_add_rrs_ref4. skip. auto => />.
 qed.
 
 
-equiv eq_h4_sub_ssr_ref4 : MHop2.sub ~ M_ref4.__sub4_ssr:
+equiv eq_spec_impl_sub_ssr_ref4 : CurveProcedures.sub ~ M_ref4.__sub4_ssr:
     f{1} = inzpRep4 fs{2} /\
     g{1} = inzpRep4 g{2}
     ==>
     res{1} = inzpRep4 res{2}.
 proof.
     proc *. inline{2} (1). wp. sp.
-    call eq_h4_sub_rsr_ref4. skip. auto => />.
+    call eq_spec_impl_sub_rsr_ref4. skip. auto => />.
 qed.
 
 
-equiv eq_h4_sub_sss_ref4 : MHop2.sub ~ M_ref4.__sub4_sss:
+equiv eq_spec_impl_sub_sss_ref4 : CurveProcedures.sub ~ M_ref4.__sub4_sss:
     f{1}   = inzpRep4 fs{2} /\
     g{1}   = inzpRep4 gs{2}
     ==>
     res{1} = inzpRep4 res{2}.
 proof.
     proc *. inline{2} (1). wp. sp.
-    call eq_h4_sub_rrs_ref4. skip. auto => />.
+    call eq_spec_impl_sub_rrs_ref4. skip. auto => />.
 qed.
 
-equiv eq_h4_mul_a24_ss_ref4 : MHop2.mul_a24 ~ M_ref4.__mul4_a24_ss:
+equiv eq_spec_impl_mul_a24_ss_ref4 : CurveProcedures.mul_a24 ~ M_ref4.__mul4_a24_ss:
     f{1}   = inzpRep4 xa{2} /\
     a24{1} = to_uint a24{2}
     ==>
     res{1} = inzpRep4 res{2}.
 proof.
     proc *. inline{2} (1). wp. sp.
-    call eq_h4_mul_a24_rs_ref4. skip. auto => />.
+    call eq_spec_impl_mul_a24_rs_ref4. skip. auto => />.
 qed.
 
-equiv eq_h4_mul_sss_ref4 : MHop2.mul ~ M_ref4.__mul4_sss:
+equiv eq_spec_impl_mul_sss_ref4 : CurveProcedures.mul ~ M_ref4.__mul4_sss:
     f{1}   = inzpRep4 xa{2} /\
     g{1}   = inzpRep4 ya{2}
     ==>
     res{1} = inzpRep4 res{2}.
 proof.
     proc *. inline{2} (1). wp. sp.
-    call eq_h4_mul_rss_ref4. skip. auto => />.
+    call eq_spec_impl_mul_rss_ref4. skip. auto => />.
 qed.
 
 
-equiv eq_h4_mul_ss_ref4 : MHop2.mul ~ M_ref4._mul4_ss_:
+equiv eq_spec_impl_mul_ss_ref4 : CurveProcedures.mul ~ M_ref4._mul4_ss_:
     f{1}   = inzpRep4 xa{2} /\
     g{1}   = inzpRep4 ya{2}
     ==>
     res{1} = inzpRep4 res{2}.
 proof.
     proc *. inline{2} (1). wp. sp.
-    call eq_h4_mul_pp_ref4. skip. auto => />.
+    call eq_spec_impl_mul_pp_ref4. skip. auto => />.
 qed.
 
 
-equiv eq_h4_sqr_ss_ref4 : MHop2.sqr ~ M_ref4._sqr4_ss_:
+equiv eq_spec_impl_sqr_ss_ref4 : CurveProcedures.sqr ~ M_ref4._sqr4_ss_:
     f{1} = inzpRep4 xa{2}
     ==>
     res{1} = inzpRep4 res{2}.
@@ -98,24 +94,24 @@ proof.
     proc *. inline{2} (1).
     unroll for{2} ^while.
     wp. sp. simplify.
-    call eq_h4_sqr_p_ref4. skip. auto => />.
+    call eq_spec_impl_sqr_p_ref4. skip. auto => />.
     move => &2.
     congr. apply Array4.ext_eq. move => H [H1] H2.
-    smt(@Array4).
+    smt(Array4.get_setE).
 qed.
 
-equiv eq_h4_sqr_s__ref4 : MHop2.sqr ~ M_ref4._sqr4_s_:
+equiv eq_spec_impl_sqr_s__ref4 : CurveProcedures.sqr ~ M_ref4._sqr4_s_:
     f{1}   = inzpRep4 x{2}
     ==>
     res{1} = inzpRep4 res{2}.
 proof.
     proc *. inline{2} (1). wp. sp.
-    call eq_h4_sqr_p_ref4. skip. auto => />.
+    call eq_spec_impl_sqr_p_ref4. skip. auto => />.
 qed.
 
 (** step 1: init points and decoding u-coordinates **)
-equiv eq_h4_init_points_ref4 :
-    MHop2.init_points ~ M_ref4.__init_points4 :
+equiv eq_spec_impl_init_points_ref4 :
+    CurveProcedures.init_points ~ M_ref4.__init_points4 :
         init{1} = inzpRep4 initr{2}
         ==>
         res{1}.`1 = inzpRep4 res{2}.`1 /\
@@ -125,15 +121,15 @@ equiv eq_h4_init_points_ref4 :
 proof.
     proc.
     wp. unroll for{2} ^while. wp. skip. move => &1 &2 H H0 H1 H2 H3 H4 H5 H6.
-    split; auto => />. rewrite /H4 /H0 /H2 /H3 /Zp_25519.one /set0_64_ /inzpRep4 => />.
+    split; auto => />. rewrite /H4 /H0 /H2 /H3 /Zp.one /set0_64_ /inzpRep4 => />.
         rewrite /valRep4 /to_list /mkseq -iotaredE => />.
-    split; auto => />. rewrite /H5  /H0 /H3 /H2 /Zp_25519.zero /set0_64_ /inzpRep4 => />.
+    split; auto => />. rewrite /H5  /H0 /H3 /H2 /Zp.zero /set0_64_ /inzpRep4 => />.
         rewrite /valRep4 /to_list /mkseq -iotaredE  => />.
-    rewrite /H6  /H0 /H3 /H2 /Zp_25519.zero /set0_64_ /inzpRep4 // /valRep4 /to_list /mkseq -iotaredE  => />.
+    rewrite /H6  /H0 /H3 /H2 /Zp.zero /set0_64_ /inzpRep4 // /valRep4 /to_list /mkseq -iotaredE  => />.
 qed.
 
-equiv eq_h4_decode_u_coordinate_base_ref4 :
-    MHop2.decode_u_coordinate_base ~ M_ref4.__decode_u_coordinate_base4:
+equiv eq_spec_impl_decode_u_coordinate_base_ref4 :
+    CurveProcedures.decode_u_coordinate_base ~ M_ref4.__decode_u_coordinate_base4:
         true
         ==>
         res{1} = inzpRep4 res{2}.
@@ -144,8 +140,8 @@ qed.
 
 
 (** step 4 : cswap **)
-equiv eq_h4_cswap_ref4 :
-    MHop2.cswap ~ M_ref4.__cswap4:
+equiv eq_spec_impl_cswap_ref4 :
+    CurveProcedures.cswap ~ M_ref4.__cswap4:
         x2{1}         = inzpRep4 x2{2}      /\
         z2{1}         = inzpRep4 z2r{2}     /\
         x3{1}         = inzpRep4 x3{2}      /\
@@ -169,9 +165,9 @@ proof.
         have lxor2 : forall (x1 x2:W64.t),  x1 `^` (x1 `^` x2) = x2.
             move=> *. rewrite xorwA xorwK xor0w //.
         rewrite !lxor1 !lxor2.
-        split. congr. apply Array4.ext_eq. smt(@Array4).
-        split. congr. apply Array4.ext_eq. smt(@Array4).
-        split. congr. apply Array4.ext_eq. smt(@Array4).
+        split. congr. apply Array4.ext_eq. smt(Array4.get_setE).
+        split. congr. apply Array4.ext_eq. smt(Array4.get_setE).
+        split. congr. apply Array4.ext_eq. smt(Array4.get_setE).
         congr. apply Array4.ext_eq. smt(@Array4).
     rcondf {1} 1 => //. wp => /=; skip.
     move => &1 &2 [#] 4!->> ??.
@@ -181,8 +177,8 @@ proof.
 qed.
 
 (** step 5 : add_and_double **)
-equiv eq_h4_add_and_double_ref4 :
-    MHop2.add_and_double ~ M_ref4.__add_and_double4:
+equiv eq_spec_impl_add_and_double_ref4 :
+    CurveProcedures.add_and_double ~ M_ref4.__add_and_double4:
         init{1} = inzpRep4 init{2}     /\
         x2{1}   = inzpRep4 x2{2}       /\
         z2{1}   = inzpRep4 z2r{2}      /\
@@ -195,30 +191,30 @@ equiv eq_h4_add_and_double_ref4 :
         res{1}.`4 = inzpRep4 res{2}.`4.
 proof.
     proc => /=.
-    call eq_h4_mul_rss_ref4.
-    call eq_h4_mul_sss_ref4.
-    call eq_h4_add_sss_ref4.
-    call eq_h4_sqr_ss__ref4.
-    call eq_h4_mul_a24_ss_ref4.
-    call eq_h4_sqr_ss__ref4.
-    call eq_h4_sub_sss_ref4.
-    call eq_h4_mul_sss_ref4.
-    call eq_h4_sub_sss_ref4.
-    call eq_h4_add_sss_ref4.
-    call eq_h4_sqr_ss__ref4.
-    call eq_h4_sqr_ss__ref4.
-    call eq_h4_mul_sss_ref4.
-    call eq_h4_mul_sss_ref4.
-    call eq_h4_add_sss_ref4.
-    call eq_h4_sub_sss_ref4.
-    call eq_h4_add_ssr_ref4.
-    call eq_h4_sub_ssr_ref4.
+    call eq_spec_impl_mul_rss_ref4.
+    call eq_spec_impl_mul_sss_ref4.
+    call eq_spec_impl_add_sss_ref4.
+    call eq_spec_impl_sqr_ss__ref4.
+    call eq_spec_impl_mul_a24_ss_ref4.
+    call eq_spec_impl_sqr_ss__ref4.
+    call eq_spec_impl_sub_sss_ref4.
+    call eq_spec_impl_mul_sss_ref4.
+    call eq_spec_impl_sub_sss_ref4.
+    call eq_spec_impl_add_sss_ref4.
+    call eq_spec_impl_sqr_ss__ref4.
+    call eq_spec_impl_sqr_ss__ref4.
+    call eq_spec_impl_mul_sss_ref4.
+    call eq_spec_impl_mul_sss_ref4.
+    call eq_spec_impl_add_sss_ref4.
+    call eq_spec_impl_sub_sss_ref4.
+    call eq_spec_impl_add_ssr_ref4.
+    call eq_spec_impl_sub_ssr_ref4.
     wp. done.
 qed.
 
 (** step 7 : montgomery_ladder **)
-equiv eq_h4_montgomery_ladder_step_ref4 :
-    MHop2.montgomery_ladder_step ~ M_ref4.__montgomery_ladder_step4:
+equiv eq_spec_impl_montgomery_ladder_step_ref4 :
+    CurveProcedures.montgomery_ladder_step ~ M_ref4.__montgomery_ladder_step4:
         inzp (to_uint k'{1}) =   inzpRep32 k{2} /\
         init'{1} = inzpRep4 init{2}             /\
         x2{1} = inzpRep4 x2{2}                  /\
@@ -235,9 +231,9 @@ equiv eq_h4_montgomery_ladder_step_ref4 :
         b2i res{1}.`5 = to_uint res{2}.`5.
 proof.
     proc => /=.
-    call eq_h4_add_and_double_ref4. wp.
-    call eq_h4_cswap_ref4. wp.
-    call eq_h4_ith_bit_ref4. skip.
+    call eq_spec_impl_add_and_double_ref4. wp.
+    call eq_spec_impl_cswap_ref4. wp.
+    call eq_spec_impl_ith_bit_ref4. skip.
     move => &1 &2 [H0] [H1] [H2] [H3] [H4] [H5] [H6] H7. split.
     auto => />. rewrite H0.
     move => [H8 H9] H10 H11 H12 H13 H14.
@@ -249,8 +245,8 @@ proof.
 qed.
 
 
-equiv eq_h4_montgomery_ladder_ref4 :
-    MHop2.montgomery_ladder ~ M_ref4.__montgomery_ladder4 :
+equiv eq_spec_impl_montgomery_ladder_ref4 :
+    CurveProcedures.montgomery_ladder ~ M_ref4.__montgomery_ladder4 :
         init'{1} = inzpRep4 u{2}                     /\
         inzp (W256.to_uint k'{1}) =  inzpRep32 k{2}
         ==>
@@ -259,7 +255,7 @@ equiv eq_h4_montgomery_ladder_ref4 :
 proof.
     proc. wp. sp.
     unroll {1} 4.
-    rcondt {1} 4. auto => />. inline MHop2.init_points.
+    rcondt {1} 4. auto => />. inline CurveProcedures.init_points.
         wp. sp. skip. auto => />.
     while(
           inzp (to_uint k'{1}) = inzpRep32 k{2}            /\
@@ -271,18 +267,18 @@ proof.
           z2{1} = inzpRep4 z2r{2}                          /\
           z3{1} = inzpRep4 z3{2}                           /\
           b2i swapped{1} = to_uint swapped{2}).
-        wp. sp. call eq_h4_montgomery_ladder_step_ref4. skip. auto => />.
+        wp. sp. call eq_spec_impl_montgomery_ladder_step_ref4. skip. auto => />.
         move => &1 &2 ctrR H H0 H1 H2. split.
         rewrite to_uintB. rewrite uleE to_uint1 => />. smt(). rewrite to_uint1 => />.
         move => H3 H4 H5 H6 H7 H8 H9 H10. split.
         rewrite ultE to_uintB. rewrite uleE to_uint1. smt().
         rewrite to_uint1 to_uint0. trivial. smt(@W64).
-    call eq_h4_montgomery_ladder_step_ref4. wp. call eq_h4_init_points_ref4. skip. done.
+    call eq_spec_impl_montgomery_ladder_step_ref4. wp. call eq_spec_impl_init_points_ref4. skip. done.
 qed.
 
 (** step 8 : iterated square **)
-equiv eq_h4_it_sqr_ref4 :
-    MHop2.it_sqr ~ M_ref4._it_sqr4_p:
+equiv eq_spec_impl_it_sqr_ref4 :
+    CurveProcedures.it_sqr ~ M_ref4._it_sqr4_p:
         f{1}            =    inzpRep4 x{2} /\
         i{1}            =    to_uint i{2}  /\
         2               <=   to_uint i{2}  /\
@@ -297,7 +293,7 @@ proof.
          ii{1}            <=   W32.modulus               /\
          0                <=   ii{1}
     ).
-    wp. call eq_h4_sqr_p_ref4. conseq(_: _ ==> h{1} = inzpRep4 x{2}).
+    wp. call eq_spec_impl_sqr_p_ref4. conseq(_: _ ==> h{1} = inzpRep4 x{2}).
     move => &1 &2 [[H][ H0] [H1] H2 [H3] H4 H5]. split. apply H5.
     rewrite /DEC_32 /rflags_of_aluop_nocf_w /ZF_of => /=.
     move => H6 H7 H8 H9. split. split. apply H9. split.
@@ -305,15 +301,15 @@ proof.
     split. move: H1. smt(). move: H2. smt(). split. rewrite H0. move => H10.
     smt(@W32). smt(@W32). skip. auto => />. wp.
     rewrite /DEC_32 /rflags_of_aluop_nocf_w /ZF_of => /=.
-    call eq_h4_sqr_p_ref4.
+    call eq_spec_impl_sqr_p_ref4.
     skip. auto => />. move => &2 H H0. split. split.
     rewrite to_uintB. rewrite uleE => />. move: H. smt().
     rewrite to_uint1 //. split. move: H0. smt(). move: H. smt().
     split. move => H1. smt(@W32). move => H1. move: H. smt().
 qed.
 
-equiv eq_h4_it_sqr_s_ref4 :
-    MHop2.it_sqr ~ M_ref4._it_sqr4_s_:
+equiv eq_spec_impl_it_sqr_s_ref4 :
+    CurveProcedures.it_sqr ~ M_ref4._it_sqr4_s_:
         f{1}            =    inzpRep4 x{2} /\
         i{1}            =    to_uint i{2}  /\
         2               <=   to_uint i{2}  /\
@@ -322,11 +318,11 @@ equiv eq_h4_it_sqr_s_ref4 :
         res{1} = inzpRep4 res{2}.
 proof.
     proc *. inline M_ref4._it_sqr4_s_. wp. sp.
-    call eq_h4_it_sqr_ref4. skip. auto => />.
+    call eq_spec_impl_it_sqr_ref4. skip. auto => />.
 qed.
 
-equiv eq_h4_it_sqr_ss_ref4 :
-        MHop2.it_sqr ~ M_ref4._it_sqr4_ss_:
+equiv eq_spec_impl_it_sqr_ss_ref4 :
+        CurveProcedures.it_sqr ~ M_ref4._it_sqr4_ss_:
         f{1}            =    inzpRep4 x{2} /\
         i{1}            =    to_uint i{2}  /\
         2               <=   to_uint i{2}  /\
@@ -337,65 +333,65 @@ equiv eq_h4_it_sqr_ss_ref4 :
 proof.
     proc *. inline M_ref4._it_sqr4_ss_.
     unroll for{2} ^while. wp. sp.
-    call eq_h4_it_sqr_ref4. skip. auto => />. move => &2 H H0. congr.
-    apply Array4.ext_eq. move => H1 [H2] H3. smt(@Array4).
+    call eq_spec_impl_it_sqr_ref4. skip. auto => />. move => &2 H H0. congr.
+    apply Array4.ext_eq. move => H1 [H2] H3. smt(Array4.get_setE).
 qed.
 
 (** step 9 : invert **)
-equiv eq_h4_invert_ref4 :
-    MHop2.invert ~ M_ref4.__invert4 :
+equiv eq_spec_impl_invert_ref4 :
+    CurveProcedures.invert ~ M_ref4.__invert4 :
         fs{1} = inzpRep4 fs{2}
         ==>
         res{1} = inzpRep4 res{2}.
 proof.
     proc.
     sp.
-    call eq_h4_mul_ss_ref4.
-    call eq_h4_sqr_s__ref4.
-    call (eq_h4_it_sqr_s_ref4). wp.
-    call eq_h4_mul_ss_ref4.
-    call eq_h4_it_sqr_s_ref4. wp.
-    call eq_h4_mul_ss_ref4.
-    call eq_h4_it_sqr_ss_ref4. wp.
-    call eq_h4_mul_ss_ref4.
-    call eq_h4_it_sqr_ss_ref4. wp.
-    call eq_h4_mul_ss_ref4.
-    call eq_h4_it_sqr_s_ref4. wp.
-    call eq_h4_mul_ss_ref4.
-    call eq_h4_it_sqr_ss_ref4. wp.
-    call eq_h4_mul_ss_ref4.
-    call eq_h4_it_sqr_ss_ref4. wp.
-    call eq_h4_mul_ss_ref4.
-    call eq_h4_it_sqr_s_ref4. wp.
-    call eq_h4_sqr_ss_ref4.
-    call eq_h4_mul_ss_ref4.
-    call eq_h4_sqr_ss_ref4.
-    call eq_h4_mul_ss_ref4.
-    call eq_h4_mul_ss_ref4.
-    call eq_h4_sqr_s__ref4.
-    call eq_h4_sqr_ss_ref4.
-    call eq_h4_sqr_ss_ref4. wp.
+    call eq_spec_impl_mul_ss_ref4.
+    call eq_spec_impl_sqr_s__ref4.
+    call (eq_spec_impl_it_sqr_s_ref4). wp.
+    call eq_spec_impl_mul_ss_ref4.
+    call eq_spec_impl_it_sqr_s_ref4. wp.
+    call eq_spec_impl_mul_ss_ref4.
+    call eq_spec_impl_it_sqr_ss_ref4. wp.
+    call eq_spec_impl_mul_ss_ref4.
+    call eq_spec_impl_it_sqr_ss_ref4. wp.
+    call eq_spec_impl_mul_ss_ref4.
+    call eq_spec_impl_it_sqr_s_ref4. wp.
+    call eq_spec_impl_mul_ss_ref4.
+    call eq_spec_impl_it_sqr_ss_ref4. wp.
+    call eq_spec_impl_mul_ss_ref4.
+    call eq_spec_impl_it_sqr_ss_ref4. wp.
+    call eq_spec_impl_mul_ss_ref4.
+    call eq_spec_impl_it_sqr_s_ref4. wp.
+    call eq_spec_impl_sqr_ss_ref4.
+    call eq_spec_impl_mul_ss_ref4.
+    call eq_spec_impl_sqr_ss_ref4.
+    call eq_spec_impl_mul_ss_ref4.
+    call eq_spec_impl_mul_ss_ref4.
+    call eq_spec_impl_sqr_s__ref4.
+    call eq_spec_impl_sqr_ss_ref4.
+    call eq_spec_impl_sqr_ss_ref4. wp.
     skip. done.
 qed.
 
 
 (** step 11 : scalarmult **)
 
-equiv eq_h4_scalarmult_internal_ref4 :
-    MHop2.scalarmult_internal ~ M_ref4.__curve25519_internal_ref4:
+equiv eq_spec_impl_scalarmult_internal_ref4 :
+    CurveProcedures.scalarmult_internal ~ M_ref4.__curve25519_internal_ref4:
         inzp(W256.to_uint k'{1}) = inzpRep32 k{2} /\
         u''{1} = inzpRep4 u{2}
         ==>
         inzp(W256.to_uint res{1}) = inzpRep4 res{2}.
 proof.
     proc.
-    call eq_h4_encode_point_ref4.
-    call eq_h4_montgomery_ladder_ref4. wp. skip.
+    call eq_spec_impl_encode_point_ref4.
+    call eq_spec_impl_montgomery_ladder_ref4. wp. skip.
     done.
 qed.
 
-equiv eq_h4_scalarmult_ref4 :
-    MHop2.scalarmult ~ M_ref4._curve25519_ref4:
+equiv eq_spec_impl_scalarmult_ref4 :
+    CurveProcedures.scalarmult ~ M_ref4._curve25519_ref4:
         inzp(W256.to_uint k'{1}) = inzpRep4 _k{2} /\
         inzp (to_uint u'{1}) = inzpRep4 _u{2}
         ==>
@@ -403,13 +399,13 @@ equiv eq_h4_scalarmult_ref4 :
         inzpRep32List (W32u8.to_list res{1}) = inzpRep4 res{2}.
 proof.
     proc.
-    call eq_h4_scalarmult_internal_ref4 => />. auto => />.
+    call eq_spec_impl_scalarmult_internal_ref4 => />. auto => />.
     move => &1 &2 H H0 H1 H2 H3 H4 H5 H6 H7. auto => />.
     rewrite -H7.
     rewrite /inzpRep32List /inzpRep4 /valRep32List. congr.
     rewrite to_uint_unpack32u8. congr. congr. smt().
-    call eq_h4_decode_u_coordinate_ref4 => />.
-    call eq_h4_decode_scalar_25519_ref4 => />.
+    call eq_spec_impl_decode_u_coordinate_ref4 => />.
+    call eq_spec_impl_decode_scalar_25519_ref4 => />.
     move => &1 &2 [H] H0 H1. split. auto => />.
     move => H2 H3 H4 H5 H6. split. auto => />.
     move => H7 H8 H9 H10. rewrite -H10.
@@ -423,8 +419,8 @@ proof.
 qed.
 
 
-lemma eq_h4_scalarmult_ptr_ref4 mem _rp _kp _up :
-    equiv [MHop2.scalarmult ~ M_ref4.__curve25519_ref4_ptr:
+lemma eq_spec_impl_scalarmult_ptr_ref4 mem _rp _kp _up :
+    equiv [CurveProcedures.scalarmult ~ M_ref4.__curve25519_ref4_ptr:
         valid_ptr (W64.to_uint _up)  32                                                          /\
         valid_ptr (W64.to_uint _kp)  32                                                          /\
         valid_ptr (W64.to_uint _rp)  32                                                          /\
@@ -444,7 +440,7 @@ proof.
     inline M_ref4.__load4 M_ref4.__store4.
     do 3! unroll for{2} ^while.
     sp. wp. auto => />.
-    call eq_h4_scalarmult_ref4. skip. auto => />.
+    call eq_spec_impl_scalarmult_ref4. skip. auto => />.
     move => &1 &2 H H0 H1 H2 H3 H4 H5 H6.
     split. split.
     rewrite H6 /inzpRep4List /inzpRep4 /valRep4 /valRep4List /load_array4.
@@ -470,22 +466,22 @@ proof.
 qed.
 
 
-equiv eq_h4_scalarmult_base_ref4 :
-    MHop2.scalarmult_base ~ M_ref4._curve25519_ref4_base:
+equiv eq_spec_impl_scalarmult_base_ref4 :
+    CurveProcedures.scalarmult_base ~ M_ref4._curve25519_ref4_base:
         inzp(W256.to_uint k'{1}) = inzpRep4 _k{2}
         ==>
         inzp(W256.to_uint res{1}) = inzpRep4 res{2}.
 proof.
     proc.
-    call eq_h4_scalarmult_internal_ref4 => />.
-    call eq_h4_decode_u_coordinate_base_ref4 => />.
-    call eq_h4_decode_scalar_25519_ref4.
+    call eq_spec_impl_scalarmult_internal_ref4 => />.
+    call eq_spec_impl_decode_u_coordinate_base_ref4 => />.
+    call eq_spec_impl_decode_scalar_25519_ref4.
     wp. skip. done.
 qed.
 
 
-lemma eq_h4_scalarmult_base_ptr_ref4 mem _rp _kp :
- equiv [MHop2.scalarmult_base ~ M_ref4.__curve25519_ref4_base_ptr:
+lemma eq_spec_impl_scalarmult_base_ptr_ref4 mem _rp _kp :
+ equiv [CurveProcedures.scalarmult_base ~ M_ref4.__curve25519_ref4_base_ptr:
         valid_ptr (W64.to_uint _rp) 32 /\
         valid_ptr (W64.to_uint _kp) 32 /\
         Glob.mem{2} = mem /\
@@ -496,7 +492,7 @@ lemma eq_h4_scalarmult_base_ptr_ref4 mem _rp _kp :
         inzp(W256.to_uint res{1}) = inzpRep4List (load_array4 Glob.mem{2} (W64.to_uint _rp)) /\ res{2} = tt].
 proof.
     proc *. inline M_ref4.__curve25519_ref4_base_ptr M_ref4.__load4 M_ref4.__store4.
-    do 2! unroll for{2} ^while. wp. sp. call eq_h4_scalarmult_base_ref4.
+    do 2! unroll for{2} ^while. wp. sp. call eq_spec_impl_scalarmult_base_ref4.
     skip. auto => />.  move => &1 &2 H H0 H1 H2. split.
     rewrite H2. rewrite /inzpRep4List /inzpRep4 /valRep4 /valRep4List /load_array4 /to_list /mkseq -iotaredE.
     congr. congr. congr. auto => />. rewrite !to_uintD_small !to_uint_small; smt(); smt().
@@ -509,8 +505,8 @@ proof.
 qed.
 
 
-lemma eq_h4_scalarmult_jade_ref4 mem _qp _np _pp:
-    equiv [MHop2.scalarmult ~ M_ref4.jade_scalarmult_curve25519_amd64_ref4:
+lemma eq_spec_impl_scalarmult_jade_ref4 mem _qp _np _pp:
+    equiv [CurveProcedures.scalarmult ~ M_ref4.jade_scalarmult_curve25519_amd64_ref4:
         valid_ptr (W64.to_uint _qp)  32                                                          /\
         valid_ptr (W64.to_uint _np)  32                                                          /\
         valid_ptr (W64.to_uint _pp)  32                                                          /\
@@ -525,15 +521,15 @@ lemma eq_h4_scalarmult_jade_ref4 mem _qp _np _pp:
         res{2} = W64.zero].
 proof.
     proc *. inline M_ref4.jade_scalarmult_curve25519_amd64_ref4. wp. sp.
-    call (eq_h4_scalarmult_ptr_ref4 mem _qp _np _pp). skip. auto => />.
+    call (eq_spec_impl_scalarmult_ptr_ref4 mem _qp _np _pp). skip. auto => />.
     move => &1 H H0 H1 H2 H3 H4 H5 H6 H7 H8 H9.
     rewrite -H9. rewrite to_uint_unpack32u8. rewrite /inzpRep32List /valRep32List.
     congr. congr. congr. smt(@W32u8).
 qed.
 
 
-lemma eq_h4_scalarmult_jade_base_ref4  mem _qp _np:
-    equiv [MHop2.scalarmult_base ~ M_ref4.jade_scalarmult_curve25519_amd64_ref4_base:
+lemma eq_spec_impl_scalarmult_jade_base_ref4  mem _qp _np:
+    equiv [CurveProcedures.scalarmult_base ~ M_ref4.jade_scalarmult_curve25519_amd64_ref4_base:
         valid_ptr (W64.to_uint _qp)  32                                                          /\
         valid_ptr (W64.to_uint _np)  32                                                          /\
         Glob.mem{2} = mem                                                                        /\
@@ -545,5 +541,5 @@ lemma eq_h4_scalarmult_jade_base_ref4  mem _qp _np:
         res{2} = W64.zero].
 proof.
     proc *. inline M_ref4.jade_scalarmult_curve25519_amd64_ref4_base. wp. sp.
-    call (eq_h4_scalarmult_base_ptr_ref4 mem _qp _np). skip. done.
+    call (eq_spec_impl_scalarmult_base_ptr_ref4 mem _qp _np). skip. done.
 qed.
